src/program_proof/tulip/paxos/res_network.v
@@ -1,0 +1,31 @@
+From Perennial.program_proof Require Import grove_prelude.
+From Perennial.program_proof.tulip.paxos Require Import base.
+
+Section res_network.
+  Context `{!paxos_ghostG Σ}.
+  (* TODO: remove this once we have real defintions for resources. *)
+  Implicit Type (γ : paxos_names).
+
+  Definition own_terminals γ (ts : gset chan) : iProp Σ.
+  Admitted.
+
+  Definition is_terminal γ (t : chan) : iProp Σ.
+  Admitted.
+
+  #[global]
+  Instance is_terminal_persistent γ t :
+    Persistent (is_terminal γ t).
+  Admitted.
+
+  Lemma terminal_update {γ ts} t :
+    own_terminals γ ts ==∗
+    own_terminals γ ({[t]} ∪ ts) ∗ is_terminal γ t.
+  Admitted.
+
+  Lemma terminal_lookup γ ts t :
+    is_terminal γ t -∗
+    own_terminals γ ts -∗
+    ⌜t ∈ ts⌝.
+  Admitted.
+
+End res_network.
